## QHO - Part 3: Coherent States Continued 

From the previous lecture, we want to calculate time evolution of a state whose hamiltonian is a Quantum Harmonic Oscillator with a resonant driving force. 

We have the following Hamiltonian:

$$
\begin{align*}
\hat{H} &= \omega (\hat{a}^\dagger \hat{a} + \frac{1}{2}) + F_0 \sin(\omega t + \phi) \hat{x} \\
&= \omega (\hat{a}^\dagger \hat{a} + \frac{1}{2}) + \beta \sin(\omega t + \phi) (\hat{a} + \hat{a}^\dagger)
\end{align*}
$$

Taking it to the interaction picture, we have:

$$
\hat{U}_0 = e^{-i \omega (\hat{a}^\dagger \hat{a} + \frac{1}{2}) t}
$$

Therefore:

$$
\begin{align*}
\hat{H}_I &= U_0^\dagger V(t) U_0 \\
&= \beta \sin(\omega t + \phi) (\hat{a} e^{-i\omega t} + \hat{a}^\dagger e^{i\omega t})
\end{align*}
$$

Finally, doing the rotating wave approximation, we get:

$$
H_I = \frac{\beta}{2i} (\hat{a} e^{i\phi} - \hat{a}^\dagger e^{-i\phi}) \\
$$

Which has the following unitary evolution operator:

$$
\hat{U} = e^{-\beta t/2 (\hat{a} e^{i\phi} - \hat{a}^\dagger e^{-i\phi})}
$$

Now, we want to apply this unitary to the $\ket{0}$ Fock state to see what happens. \
However, we can't just trivially break up this exponential into two pieces, because remember that

$$
e^{X + Y} = e^{X} e^{Y} \leftarrow [X, Y] = 0
$$

Which isn't true in our case because **$\hat{a}$ and $\hat{a}^\dagger$ don't commute.**
Therefore we have to use the Baker-Campbell-Hausdorff (BCH) formula.

--- 
Quick reminder about the BCH formula, we want to find the solution $Z$ to the equation

$$
e^{X} e^{Y} = e^{Z}
$$

$$
Z = X + Y + \frac{1}{2} [X, Y] + \frac{1}{12} [X, [X, Y]] - \frac{1}{12} [Y, [X, Y]] + \cdots
$$

---

In our case, with $X = \frac{\beta t}{2} e^{-i\phi} \hat{a}^\dagger$ and $Y = -\frac{\beta t}{2} e^{i\phi} \hat{a}$, calculating $[X, Y]$, we get:
$$
[X, Y] = -(\frac{\beta t}{2})^2 [\hat{a}^\dagger, \hat{a}] = (\frac{\beta t}{2})^2
$$

Which shows that $[X, [X, Y]] = 0$ and $[Y, [X, Y]] = 0$. 

Therefore, the BCH formula truncates to:

$$
\begin{align*}
\hat{U} &= e^{X + Y} = e^{-\frac{1}{2} [X, Y]} e^{X} e^{Y} \\
&= e^{-\frac{1}{2} (\frac{\beta t}{2})^2} e^{\frac{\beta t}{2} e^{-i\phi} \hat{a}^\dagger} e^{-\frac{\beta t}{2} e^{i\phi} \hat{a}} \\
\end{align*}
$$

Now, step-by-step, let's see how this operator acts on $\ket{0}$:

Step 1.

$$
\begin{align*}
e^{-\frac{\beta t}{2} e^{i\phi} \hat{a}} \ket{0} &= \sum_{n=0}^\infty \frac{1}{n!} (-\frac{\beta t}{2} e^{i\phi})^n \hat{a}^n \ket{0} \\
&= \ket{0}
\end{align*}
$$

Because all the $n \neq 0$ terms for $\hat{a}^n \ket{0} = 0$. \
(See how we chose our $X$ and $Y$ wisely here to ease our calculations as every other factor in the sum goes to zero because of the $\hat{a}$ operators; due to the nature of the $X+Y$ sum, we could've done it either way.)

Step 2.

$$
\begin{align*}
e^{\frac{\beta t}{2} e^{-i\phi} \hat{a}^\dagger} \ket{0} &= \sum_{n=0}^{\infty} (\frac{\beta t}{2} e^{-i\phi})^n \frac{(\hat{a}^\dagger)^n}{n!} \ket{0} \\
&= \sum_{n=0}^{\infty} (\frac{\beta t}{2} e^{-i\phi})^n \frac{\ket{n}}{\sqrt{n!}}  \\
&= \ket{\frac{\beta t}{2} e^{-i\phi}} \\
&= \ket{\alpha}
\end{align*}
$$

Where for the last line, we used the formula for the coherent state. We'll repeat it here just as a reminder:

$$
\ket{\alpha} = \sum_{n=0}^{\infty} \frac{\alpha^n}{\sqrt{n!}} \ket{n}
$$

Step 3 (final step).

$$
\hat{U} \ket{0} = e^{-\frac{1}{2} (\frac{\beta t}{2})^2} \ket{\alpha} \cong \ket{\alpha}
$$

So this time evolution operator which came from applying a resonance force to the harmonic oscillator actually creates a coherent state when it's applied to the $\ket{0}$ state. 

### Expectation Values

$$
\braket{ \hat{x}(t) } = \sqrt{\frac{2\hbar}{m \omega}} \times Re(\alpha) = \frac{F_0}{2m \omega} t \times \cos(\phi)
$$

$$
\braket{ \hat{p}(t) } = \sqrt{2\hbar m \omega} \times Im(\alpha) = \frac{F_0}{2} t \times \sin(\phi)
$$

Since we had set $\beta = \frac{F_0}{2m \omega}$ in the previous lecture.

But this is still not time dependent in the way we want it, because if we apply it for a bigger $t$, we'll only increase the amplitude of $\hat{x}$ and $\hat{p}$, but we want to see the oscillations.

Therefore, we need to see them in the lab frame, which means we need to do the following transformation:

$$
\ket{\psi} = U_0 \ket{\psi_I} \\
\Rightarrow \ket{\psi(t)} = U_0 (\hat{U} \ket{0}) = \ket{\alpha} = \ket{\frac{\beta t}{2} e^{-i(\omega t + \phi)}}
$$

So now our expectation values become:

$$
\braket{ \hat{x}(t) } = \sqrt{\frac{2\hbar}{m \omega}} \times Re(\frac{\beta t}{2} e^{-i(\omega t + \phi)}) = \frac{F_0}{2m \omega} t \times \cos(\omega t + \phi)
$$

And for momentum:

$$
\braket{ \hat{p}(t) } = \sqrt{2\hbar m \omega} \times Im(\frac{\beta t}{2} e^{-i(\omega t + \phi)}) = \frac{F_0}{2} t \times \sin(\omega t + \phi)
$$

(This is what gave rise to the spiral forms in the homework graphs.)

Let's look at our $\hat{U}$ again:

$$
\begin{align*}
\hat{U} &= e^{-\frac{1}{2} (\frac{\beta t}{2})^2} e^{\frac{\beta t}{2} e^{-i\phi} \hat{a}^\dagger} e^{-\frac{\beta t}{2} e^{i\phi} \hat{a}} \\
&= e^{(\hat{a}^\dagger \alpha - \hat{a} \alpha^{*})} \equiv \hat{D}(\alpha)
\end{align*}
$$

Where $\hat{D}(\alpha)$ is called the displacement operator and it operate such that:

$$
\hat{D}(\alpha) \ket{0} = \ket{ \alpha }
$$

