# Quantum Harmonic Oscillators - Part 2

Our Hamiltonian for the Quantum Harmonic Oscillator is:

$$
\hat{H} = \frac{\hat{p}^2}{2m} + \frac{m \omega^2}{2} \hat{x}^2 \\
$$

Using the following ladder operators:

$$
\hat{a} = \sqrt{\frac{m \omega}{2 \hbar}} (\hat{x} + \frac{i}{m \omega} \hat{p}) \\
\, \\
\hat{a}^\dagger = \sqrt{\frac{m \omega}{2 \hbar}} (\hat{x} - \frac{i}{m \omega} \hat{p})
$$

We can write the Hamiltonian as:

$$
\hat{H} = \hbar \omega \big( \hat{a}^\dagger \hat{a} + \frac{1}{2} \big)
$$

Defining the number operator as:

$$
\hat{N} = \hat{a}^\dagger \hat{a} \\
\, \\
\hat{N} \ket{n} = n \ket{n}
$$

The Hamiltonian can also be written as:

$$
\hat{H} = \hbar \omega \big( \hat{N} + \frac{1}{2} \big)
$$

This is a time-independent Hamiltonian, so we can write its evolution operator as:

$$
\begin{align*}
\hat{U} &= e^{-i \hat{H} t / \hbar} \\
&= e^{-i \omega \big( \hat{N} + \frac{1}{2} \big) t} \\
\text{Since } & \hat{N} \text{ is a diagonal operator, } \\
&= e^{-i \omega \big( \hat{n} + \frac{1}{2} \big) t} \\
\text{We can also write} & \text{ it in terms of its eigenvectors:} \\
&= \sum_{n=0}^{\infty} e^{-i \omega \big( n + \frac{1}{2} \big) t} \ket{n} \bra{n} \\
\end{align*}
$$



## Expectation Values of Operators on Fock States

What are these?

$$
\braket{ \hat{x} } = \braket{ n | \hat{x} | n }
$$

$$
\braket{ \hat{p} } = \braket{ n | \hat{p} | n }
$$

We know that:

$$
\hat{a} = \sqrt{\frac{m \omega}{2 \hbar}} (\hat{x} + \frac{i}{m \omega} \hat{p})
$$

Therefore:

$$
\sqrt{\frac{2 \hbar}{m \omega}}(\hat{a} + \hat{a}^\dagger) = 2 \hat{x} \\
\Rightarrow \hat{x} = \sqrt{\frac{ \hbar}{2m \omega}}(\hat{a} + \hat{a}^\dagger)
$$

And

$$
\sqrt{\frac{2 \hbar}{m \omega}}(\hat{a} - \hat{a}^\dagger) = 2 i \hat{p} \\
$$

Therefore:
$$
\hat{p} = -i \sqrt{\frac{ \hbar m \omega}{2}}(\hat{a} - \hat{a}^\dagger)
$$

So we can simply see that:

$$
\braket{ \hat{x} } = 0 \\
\braket{ \hat{p} } = 0
$$

And for the uncertainties of position and momentum:

$$
\Delta x = \sqrt{\braket{ \hat{x}^2 } - \braket{ \hat{x} }^2} = \sqrt{\frac{\hbar}{2 m \omega} (2n + 1)}
$$

$$
\Delta p = \sqrt{\braket{ \hat{p}^2 } - \braket{ \hat{p} }^2} = \sqrt{\frac{\hbar m \omega}{2} (2n + 1)}
$$

$$
\Delta x \Delta p = \frac{\hbar}{2} (2n + 1)
$$

_Throwing shade on Griffiths_:

Plotting the position and momentum of these Fock states, we see that they're both always at the origin, so the plot will be a filled circle whose radius is determined by our uncertainty.

But Griffiths says that when we increase $n$, because of the classical correspondence principle, we will see that the Fock states will spend more and more time at the boundaries, just like a classical oscillator; but these are stationary states! We can't really expect them to oscillate.

So now we're going to inspect something that will correspond to our classical intuition on the classical oscillator, the coherent state.

<br/>

## Coherent States

Let's think before we jump. We know that we're going to introduce a new type of state that isn't stationary, therefore it needs to be in some sort of **superposition** of our Fock states.

In the classical case, we know that our oscillator has a **fixed** number $a =\sqrt{\frac{m\omega}{2}} (x + \frac{i}{m \omega} p)$ all throughout its oscillation, we expect that our quantum analogue will be an **eigenstate** of $\hat{a}$.

Mathematically, we can write this as:
$$
\hat{a} \ket{ \alpha } = \alpha \ket{ \alpha }
$$

Since the lowering operator $\hat{a}$ acting on Fock states is only ever going to give us _different_ states, they won't be the eigenstates, but an infinite sum of them will.

Why infintite? Because if you lower any of the states in a finite sum of states, you will definitely get a state that isn't the original sum.

So, we will make a _guess_ of what our state is supposed to look like (We will include time dependence later):

$$
\ket{ \alpha } = C \times \sum_{n=0}^{\infty} \frac{\lambda^n}{\sqrt{n!}} \ket{ n }
$$

Where $C$ is just a normalization factor.

Putting this in the defining equation of the coherent state, we get:

$$
\begin{align*}
\hat{a} \ket{ \alpha } &= C \times \sum_{n=1}^{\infty} \frac{\lambda^n}{\sqrt{(n-1)!}} \ket{ n-1 } \\
&= \lambda \times \big( C \times \sum_{n=1}^{\infty} \frac{\lambda^{n-1}}{\sqrt{(n-1)!}} \ket{ n-1 } \big) \\
&\stackrel{m = n+1}{=} \lambda \times \big( C \times \sum_{m=0}^{\infty} \frac{\lambda^{m}}{\sqrt{m!}} \ket{ m } \big) \\
&= \lambda \ket{ \alpha }
\end{align*}
$$

(In the second line, after applying $\hat{a}$ to all of the terms, we see that the sum starts from $n=1$ because $\hat{a}\ket{0} = 0$)

So we see that $\alpha$ is indeed an eigenstate of $\hat{a}$! And its eigenvector is whatever number we put in for $\lambda$, so for the sake of our sanity, let's call that $\alpha$ as well from now on:

$$
\sum_{n=0}^{\infty} \frac{\alpha^n}{\sqrt{n!}} \ket{ n } = \alpha \ket{ \alpha }
$$

Let's now find our normalization factor $C$:

$$
\begin{align*}
\langle \alpha \ket{ \alpha } = 1 &= \big( \sum_{m=0}^{\infty} \frac{\alpha^m}{\sqrt{m!}} \bra{ m } \big) \big( \sum_{n=0}^{\infty} \frac{\alpha^n}{\sqrt{n!}} \big( \ket{n} ) \\
& \stackrel{\braket{ m | n } = \delta_{m,n}}{=} |C|^2 \sum_{n=0}^{\infty} \frac{(|\alpha|^2)^n}{n!} \\
& \stackrel{Taylor}{=} |C|^2 e^{|\alpha|^2} = 1
\end{align*}
$$

Which gives us:

$$
C = e^{-|\alpha|^2/2}
$$

So the final form of our **coherent state** is:

$$
 \ket{ \alpha } = e^{-|\alpha|^2/2} \sum_{n=0}^{\infty} \frac{\alpha^n}{\sqrt{n!}} \ket{n}
$$

And $\alpha$ can be anything, even complex numbers! \
Note that this is only possible because $\hat{a}$ is **NOT** a Hermitian operator, meaning that $\hat{a} \neq \hat{a}^\dagger$, so we can have complex eigenvalues.

### Expectation values of operators on coherent states

First, let's figure out what the raising operator $\hat{a}^\dagger$ does to our coherent state:
$$
(\hat{a} \ket{\alpha} )^\dagger = (\alpha \ket{ \alpha })^\dagger \\
\Rightarrow \bra{ \alpha } \hat{a}^\dagger = \alpha^{*} \bra{ \alpha }
$$

So now we see:

$$
\begin{align*}
\braket{ \hat{x} } &= \braket{ \alpha | \hat{x} | \alpha } \\
&= \sqrt{\frac{ \hbar}{2m \omega}} \braket{ \alpha |\hat{a} + \hat{a}^\dagger | \alpha } \\
&= \sqrt{\frac{ \hbar}{2m \omega}} (\alpha \braket{ \alpha | \alpha } + \braket{ \alpha |  a^\dagger | \alpha }) \\
&= \sqrt{\frac{ \hbar}{2m \omega}} (\alpha + \alpha^{*}) \\
&= \sqrt{\frac{ \hbar}{2m \omega}} \times Re(\alpha) \\
\end{align*}
$$

And, similarly:

$$
\begin{align*}
\braket{ \hat{p} } &= \braket{ \alpha | \hat{p} | \alpha } \\
&= -i \sqrt{\frac{\hbar m \omega}{2}} \braket{ \alpha |\hat{a} - \hat{a}^\dagger | \alpha } \\
&= -i \sqrt{\frac{\hbar m \omega}{2}} (\alpha - \alpha^{*}) \\
&= \sqrt{2\hbar m \omega} \times Im(\alpha)
\end{align*}
$$

And the uncertainties for these operators on the coherent states are:

$$
\Delta x = \sqrt{\frac{\hbar}{2m\omega}}
$$

$$
\Delta x = \sqrt{\frac{\hbar m \omega}{2}}
$$

Therefore:

$$
\Delta x \Delta p = \frac{\hbar}{2}
$$

This means that these states have the minimum uncertainty allowed by Quantum Mechanics. \
(Actually Heisenberg found them precisely because he was trying to find the minimum uncertainty states)

### Time dependence of coherent states

If we plot these coherent states on an $x-p$ graph, we see that they're stationary in a point $|\alpha|$ away from the origin, but they're not moving, because they have no time dependence.

Remembering that the Hamiltonian for the Quantum Harmonic Oscillator is:

$$
H = \hbar \omega (\hat{a}^\dagger \hat{a} + \frac{1}{2})
$$

Our evolution operator becomes:

$$
\hat{U}(t) = e^{-i\omega (\hat{a}^\dagger \hat{a} + \frac{1}{2}) t} = e^{-i\omega (n + \frac{1}{2}) t}
$$

Applying it to the coherent state:

$$
\begin{align*}
\ket{\alpha (t) } &= \hat{U}(t) \ket{\alpha} \\
&= e^{-i\omega (\hat{a}^\dagger \hat{a} + \frac{1}{2}) t} \Big( e^{-|\alpha|^2/2} \sum_{n=0}^{\infty} \frac{\alpha^n}{\sqrt{n!}} \ket{n} \Big) \\
&= e^{-|\alpha|^2/2} \sum_{n=0}^{\infty} \frac{\alpha^n e^{-i\omega (n + \frac{1}{2})}}{\sqrt{n!}} \ket{n} \\
&= e^{-i\omega t/2} \big( e^{-|\alpha|^2/2} \sum_{n=0}^{\infty} \frac{(\alpha e^{-i\omega t})^n }{\sqrt{n!}}  \ket{n} \big) \\
&= e^{-i\omega t/2} \ket{\alpha e^{-i \omega t} }
\end{align*}
$$

So basically our new time-dependent coherent states will have an $\alpha$ that's also time dependent!

Doing the same calculations for the expectation values of operators we get:

$$
\braket{ \hat{x} } = \sqrt{\frac{ \hbar}{2m \omega}} \times Re(\alpha) \times \cos(\omega t)
$$

And,

$$
\braket{ \hat{p} } = \sqrt{2\hbar m \omega} \times Im(\alpha) \times \sin(\omega t)
$$

We see that by having a $\sin$ and a $\cos$ in our position and momentum, they will start to move on to form a circle on the $x-p$ diagram!

Note that the uncertainty is the same for all coherent states, and we will get the same value that we got for the "stationary" coherent states.

### How to make a coherent state?

If we were doing it classically, we would do it by applying a resonant (same frequency) force $F_0 \sin(\omega t + \phi)$ to the oscillator, but since we're dealing with hamiltonians in Quantum Mechanics, we need to do it with a potential energy.

So our new Hamiltonian will be (omitting an $\hbar$ factor):

$$
\begin{align*}
\hat{H} &= \omega (\hat{a}^\dagger \hat{a} + \frac{1}{2}) + F_0 \sin(\omega t + \phi) \hat{x} \\
&= \omega (\hat{a}^\dagger \hat{a} + \frac{1}{2}) + F_0 \sqrt{\frac{\hbar}{2 m \omega}} \sin(\omega t + \phi) (\hat{a} + \hat{a}^\dagger) \\
&= \omega (\hat{a}^\dagger \hat{a} + \frac{1}{2}) + \beta \sin(\omega t + \phi) (\hat{a} + \hat{a}^\dagger)
\end{align*}
$$

Where $\beta = F_0 \sqrt{\frac{\hbar}{2 m \omega}}$.

So now, we want to find the evolution of a system whose hamiltonian is $\hat{H}$, which is composed of a time-independent part and a time-dependent part. What do we do? 

**Interaction Picture!**

$$
\hat{U}_0 = e^{-i \omega (\hat{a}^\dagger \hat{a} + \frac{1}{2}) t}
$$
(Which as usual cancels out the time-independent part of the hamiltonian, and leaves us with the time-dependent part)

$$
\begin{align*}
\hat{H}_I &= \hat{U}_0^\dagger \hat{H} \hat{U}_0  \\
&= \beta \sin(\omega t + \phi) e^{iw (\hat{a}^\dagger \hat{a} + \frac{1}{2}) t} (\hat{a} + \hat{a}^\dagger) e^{-iw (\hat{a}^\dagger \hat{a} + \frac{1}{2}) t} \\
&= \beta \sin(\omega t + \phi) (\hat{a} e^{-i\omega t} + \hat{a}^\dagger e^{i\omega t})
\end{align*}
$$

(The last line makes use of an identity which is easily provable using the taylor series form of the matrix exponentials.)

---
Those identities being:

For the QHO hamtiloninan:

$$
H_0 = \omega(\hat{a}^\dagger \hat{a} + \frac{1}{2})
$$

We have:

$$
e^{iH_0t} \hat{a} e^{-iH_0t} = \hat{a} e^{-i\omega t}
$$

$$
e^{iH_0t} \hat{a}^\dagger e^{-iH_0t} = \hat{a}^\dagger e^{i\omega t}
$$

---

Now, we have a hamiltonian which the product of a $\sin$ and $e^{i\omega t}$, what should we do? 

**Rotating Wave Approximation!** \
($2 \omega$ is a really high frequency that we could approximate it as being constant.)

$$
\begin{align*}
\hat{H}_I &= \beta \sin(\omega t + \phi) (\hat{a} e^{-i\omega t} + \hat{a}^\dagger e^{i\omega t}) \\
&= \beta \frac{e^{i (\omega t + \phi)} - e^{-i (\omega t + \phi)}}{2i} (\hat{a} e^{-i\omega t} + \hat{a}^\dagger e^{i\omega t}) \\
& \stackrel{RWA}{=} \frac{\beta}{2i} (\hat{a} e^{i\phi} - \hat{a}^\dagger e^{-i\phi}) \\
\end{align*}
$$

This hamiltonian is now time-independent, so we can easily exponentiate to find the evolution operator:

$$
\hat{U} = e^{-\beta t/2 (\hat{a} e^{i\phi} - \hat{a}^\dagger e^{-i\phi})}
$$